Add solution for Pset5

pset5/Pset5.v
@@ -4,7 +4,424 @@ Require Import Frap Pset5Sig.
  * which contains the instructions.
  *)
 
+Fixpoint genbuf (n:nat) : list nat :=
+  match n with
+    | O => nil
+    | S q => 1 :: (genbuf q)
+  end.
+
+Definition non_null (n:nat) := exists (n_1:nat), n = S n_1.
+
+Definition pdcs2_inv
+           (s : threaded_state (sharedWithLock pdcs_global_state)
+                               (stateWithLock pd_thread * stateWithLock cs_thread)) :=
+  exists (a b c: nat),
+  s.(Shared).(SharedOrig).(cnt) = a /\
+  s.(Shared).(SharedOrig).(buf) = genbuf b /\
+  s.(Shared).(SharedOrig).(acc) = c /\
+  ((
+    (
+      (s.(Shared).(Lock) = false /\ s.(Private) = (Alock, Alock) /\ non_null a) \/
+      (s.(Shared).(Lock) = true /\ s.(Private) = (Aprivate DecCount, Alock) /\ non_null a) \/
+      (s.(Shared).(Lock) = true /\ s.(Private) = (Aunlock, Alock)) \/
+      (s.(Shared).(Lock) = false /\ s.(Private) = (Aprivate CheckCount, Alock)) \/
+      (s.(Shared).(Lock) = true /\ s.(Private) = (Alock, Aprivate Pop) /\ non_null a) \/
+      (s.(Shared).(Lock) = true /\ s.(Private) = (Alock, Aunlock) /\ non_null a) \/
+      (s.(Shared).(Lock) = true /\ s.(Private) = (Aprivate CheckCount, Aprivate Pop)) \/
+      (s.(Shared).(Lock) = true /\ s.(Private) = (Aprivate CheckCount, Aunlock))
+    ) /\ (
+      a + b + c = PRD_COUNT
+    )
+  ) \/ (
+    (
+      (s.(Shared).(Lock) = true /\ s.(Private) = (Aprivate Push, Alock)) \/
+      (s.(Shared).(Lock) = true /\ s.(Private) = (Alock, Aprivate (Acc 1)) /\ non_null a) \/
+      (s.(Shared).(Lock) = true /\ s.(Private) = (Aprivate CheckCount, Aprivate (Acc 1)))
+    ) /\ (
+      S (a + b + c) = PRD_COUNT
+    )
+  )).
+
+Theorem pdcs2_ok_complete: invariantFor pdcs2_sys pdcs2_inv.
+Proof.
+  refine (invariant_induction pdcs2_sys pdcs2_inv _ _).
+  (* Initial state *)
+    intros s_init s_init_value.
+    cases s_init_value.
+    invert H.
+    invert H0.
+    refine (ex_intro _ PRD_COUNT (ex_intro _ O (ex_intro _ O _))).
+    refine (conj _ (conj _ (conj _ _))).
+    equality.
+    equality.
+    equality.
+    refine (or_introl (conj (or_intror (or_intror (or_intror (or_introl (conj _ _))))) _)).
+    equality.
+    equality.
+    equality.
+  (* Induction *)
+    intros s1 s1_inv s2 s2_transition.
+    destruct s1_inv as [ a s1_inv ].
+    destruct s1_inv as [ b s1_inv ].
+    destruct s1_inv as [ c s1_inv ].
+    destruct s1_inv as [ cnt_a s1_inv ].
+    destruct s1_inv as [ cnt_b s1_inv ].
+    destruct s1_inv as [ cnt_c s1_inv ].
+    cases s1_inv.
+      destruct H as [ H sum_abc ].
+      cases H.
+    (* Alock, Alock *)
+        destruct H as [ main_lock rest ].
+        destruct rest as [ state a_neq_0 ].
+        cases s2_transition.
+        (* AstepN1 *)
+          discriminate state.
+        (* AstepN2 *)
+          discriminate state.
+        (* AstepLock1 *)
+          refine (ex_intro _ a (ex_intro _ b (ex_intro _ c (conj cnt_a (conj cnt_b (conj cnt_c _)))))).
+          refine (or_introl (conj (or_intror (or_introl _)) sum_abc)).
+          invert H.
+          invert state.
+          refine (conj _ (conj _ _)).
+          equality.
+          equality.
+          exact a_neq_0.
+        (* AstepLock2 *)
+          refine (ex_intro _ a (ex_intro _ b (ex_intro _ c (conj cnt_a (conj cnt_b (conj cnt_c _)))))).
+          refine (or_introl (conj (or_intror (or_intror (or_intror (or_intror (or_introl _))))) sum_abc)).
+          invert H.
+          invert state.
+          refine (conj _ (conj _ _)).
+          equality.
+          equality.
+          exact a_neq_0.
+        (* AstepUnlock1 *)
+          discriminate state.
+        (* AstepUnlock2 *)
+          discriminate state.
+      cases H.
+    (* Aprivate DecCount, Alock *)
+        destruct H as [ main_lock rest ].
+        destruct rest as [ state a_neq_0 ].
+        cases s2_transition.
+        (* AstepN1 *)
+          refine (ex_intro _ (pred a) (ex_intro _ b (ex_intro _ c _))).
+          invert H.
+          invert state.
+          refine (conj _ (conj _ (conj _ _))).
+          equality.
+          exact cnt_b.
+          equality.
+          refine (or_intror (conj (or_introl (conj main_lock _)) sum_abc)).
+          invert state.
+          equality.
+          discriminate state.
+        (* AstepN2 *)
+          discriminate state.
+        (* AstepLock1 *)
+          discriminate state.
+        (* AstepLock2 *)
+          discriminate main_lock.
+        (* AstepUnlock1 *)
+          discriminate state.
+        (* AstepUnlock2 *)
+          discriminate state.
+      cases H.
+    (* Aunlock, Alock *)
+        destruct H as [ main_lock state ].
+        cases s2_transition.
+        (* AstepN1 *)
+          discriminate state.
+        (* AstepN2 *)
+          discriminate state.
+        (* AstepLock1 *)
+          discriminate state.
+        (* AstepLock2 *)
+          discriminate main_lock.
+        (* AstepUnlock1 *)
+          refine (ex_intro _ a (ex_intro _ b (ex_intro _ c (conj cnt_a (conj cnt_b (conj cnt_c _)))))).
+          refine (or_introl (conj (or_intror (or_intror (or_intror (or_introl (conj _ _))))) sum_abc)).
+          equality.
+          invert H.
+          invert state.
+          equality.
+        (* AstepUnlock2 *)
+          discriminate state.
+      cases H.
+    (* Aprivate CheckCount, Alock *)
+        destruct H as [ main_lock state ].
+        cases s2_transition.
+        (* AstepN1 *)
+          invert state.
+          invert H.
+          refine (ex_intro _ (S c) (ex_intro _ b (ex_intro _ a (conj _ (conj cnt_b (conj _ _)))))).
+          equality.
+          equality.
+          refine (or_introl (conj (or_introl (conj main_lock (conj (eq_refl _) _))) sum_abc)).
+          exact (ex_intro _ c (eq_refl (S c))).
+        (* AstepN2 *)
+          discriminate state.
+        (* AstepLock1 *)
+          discriminate state.
+        (* AstepLock2 *)
+          invert state.
+          invert H.
+          refine (ex_intro _ (cnt sh) (ex_intro _ b (ex_intro _ (acc sh) (conj _ (conj cnt_b (conj _ _)))))).
+          equality.
+          equality.
+          refine (or_introl (conj (or_intror (or_intror (or_intror (or_intror (or_intror
+              (or_intror (or_introl (conj _ _)))))))) sum_abc)).
+          equality.
+          equality.
+        (* AstepUnlock1 *)
+          discriminate state.
+        (* AstepUnlock2 *)
+          discriminate state.
+      cases H.
+    (* Alock, Aprivate Pop *)
+        destruct H as [ main_lock rest ].
+        destruct rest as [ state a_neq_0 ].
+        cases s2_transition.
+        (* AstepN1 *)
+          discriminate state.
+        (* AstepN2 *)
+          invert state.
+          invert H.
+          cases b.
+          discriminate cnt_b.
+          refine (ex_intro _ c (ex_intro _ b (ex_intro _ a (conj _ (conj _ (conj _ _)))))).
+          equality.
+          simpl.
+          simpl in cnt_b.
+          exact (f_equal (fun (l:list nat) => tl l) cnt_b).
+          equality.
+          refine (or_intror (conj (or_intror (or_introl (conj main_lock (conj _ a_neq_0)))) _)).
+          simpl in cnt_b.
+          simpl.
+          exact (f_equal (fun (l:list nat) => (Alock, Aprivate (Acc (hd 1 l)))) cnt_b).
+          simpl in sum_abc.
+          rewrite <- (plus_Sn_m (c + b) a).
+          rewrite (plus_n_Sm c b).
+          exact sum_abc.
+        (* AstepLock1 *)
+          discriminate main_lock.
+        (* AstepLock2 *)
+          discriminate state.
+        (* AstepUnlock1 *)
+          discriminate state.
+        (* AstepUnlock2 *)
+          discriminate state.
+      cases H.
+    (* Alock, Aunlock *)
+        destruct H as [ main_lock rest ].
+        destruct rest as [ state a_neq_0 ].
+        cases s2_transition.
+        (* AstepN1 *)
+          discriminate state.
+        (* AstepN2 *)
+          discriminate state.
+        (* AstepLock1 *)
+          discriminate main_lock.
+        (* AstepLock2 *)
+          discriminate state.
+        (* AstepUnlock1 *)
+          discriminate state.
+        (* AstepUnlock2 *)
+          invert state.
+          invert H.
+          refine (ex_intro _ (cnt sh) (ex_intro _ b (ex_intro _ (acc sh) (conj _ (conj cnt_b (conj _ _)))))).
+          equality.
+          equality.
+          refine (or_introl (conj (or_introl (conj _ (conj _ a_neq_0))) sum_abc)).
+          equality.
+          equality.
+      cases H.
+    (* Aprivate CheckCount, Aprivate Pop *)
+        destruct H as [ main_lock state ].
+        cases s2_transition.
+        (* AstepN1 *)
+          invert state.
+          invert H.
+          refine (ex_intro _ (S c) (ex_intro _ b (ex_intro _ a (conj _ (conj cnt_b (conj _ _)))))).
+          equality.
+          equality.
+          refine (or_introl (conj (or_intror (or_intror (or_intror (or_intror (or_introl
+              (conj main_lock (conj (eq_refl _) _))))))) sum_abc)).
+          exact (ex_intro _ c (eq_refl (S c))).
+        (* AstepN2 *)
+          invert state.
+          invert H.
+          cases b.
+          discriminate cnt_b.
+          refine (ex_intro _ c (ex_intro _ b (ex_intro _ a (conj _ (conj _ (conj _ _)))))).
+          equality.
+          simpl.
+          simpl in cnt_b.
+          exact (f_equal (fun (l:list nat) => tl l) cnt_b).
+          equality.
+          refine (or_intror (conj (or_intror (or_intror (conj main_lock _))) _)).
+          simpl in cnt_b.
+          simpl.
+          exact (f_equal (fun (l:list nat) => (Aprivate CheckCount, Aprivate (Acc (hd 1 l)))) cnt_b).
+          simpl in sum_abc.
+          rewrite <- (plus_Sn_m (c + b) a).
+          rewrite (plus_n_Sm c b).
+          exact sum_abc.
+        (* AstepLock1 *)
+          discriminate state.
+        (* AstepLock2 *)
+          discriminate state.
+        (* AstepUnlock1 *)
+          discriminate state.
+        (* AstepUnlock2 *)
+          discriminate state.
+    (* Aprivate CheckCount, Aunlock *)
+        destruct H as [ main_lock state ].
+        cases s2_transition.
+        (* AstepN1 *)
+          invert state.
+          invert H.
+          refine (ex_intro _ (S c) (ex_intro _ b (ex_intro _ a (conj _ (conj cnt_b (conj _ _)))))).
+          equality.
+          equality.
+          refine (or_introl (conj (or_intror (or_intror (or_intror (or_intror (or_intror (or_introl
+              (conj main_lock (conj (eq_refl _) _)))))))) sum_abc)).
+          exact (ex_intro _ c (eq_refl (S c))).
+        (* AstepN2 *)
+          discriminate state.
+        (* AstepLock1 *)
+          discriminate state.
+        (* AstepLock2 *)
+          discriminate state.
+        (* AstepUnlock1 *)
+          discriminate state.
+        (* AstepUnlock2 *)
+          invert state.
+          invert H.
+          refine (ex_intro _ (cnt sh) (ex_intro _ b (ex_intro _ (acc sh) (conj _ (conj cnt_b (conj _ _)))))).
+          equality.
+          equality.
+          refine (or_introl (conj (or_intror (or_intror (or_intror (or_introl (conj _ _))))) sum_abc)).
+          equality.
+          equality.
+      destruct H as [ H sum_abc ].
+      cases H.
+    (* Aprivate Push, Alock *)
+        destruct H as [ main_lock state ].
+        cases s2_transition.
+        (* AstepN1 *)
+          invert state.
+          invert H.
+          refine (ex_intro _ c (ex_intro _ (S b) (ex_intro _ a (conj _ (conj _ (conj _ _)))))).
+          equality.
+          simpl.
+          rewrite <- cnt_b.
+          equality.
+          equality.
+          refine (or_introl (conj (or_intror (or_intror (or_introl (conj main_lock (eq_refl _))))) _)).
+          simpl in sum_abc.
+          rewrite <- (plus_Sn_m (c + b) a) in sum_abc.
+          rewrite (plus_n_Sm c b) in sum_abc.
+          exact sum_abc.
+        (* AstepN2 *)
+          discriminate state.
+        (* AstepLock1 *)
+          discriminate state.
+        (* AstepLock2 *)
+          discriminate main_lock.
+        (* AstepUnlock1 *)
+          discriminate state.
+        (* AstepUnlock2 *)
+          discriminate state.
+      cases H.
+    (* Alock, Aprivate (Acc 1) *)
+        destruct H as [ main_lock rest ].
+        destruct rest as [ state a_neq_0 ].
+        cases s2_transition.
+        (* AstepN1 *)
+          discriminate state.
+        (* AstepN2 *)
+          invert state.
+          invert H.
+          refine (ex_intro _ c (ex_intro _ b (ex_intro _ (S a) (conj _ (conj cnt_b (conj _ _)))))).
+          equality.
+          rewrite (plus_comm a 1).
+          equality.
+          refine (or_introl (conj (or_intror (or_intror (or_intror (or_intror (or_intror
+              (or_introl (conj main_lock (conj (eq_refl _) a_neq_0)))))))) _)).
+          simpl in sum_abc.
+          rewrite (plus_n_Sm (c + b) a) in sum_abc.
+          exact sum_abc.
+        (* AstepLock1 *)
+          discriminate main_lock.
+        (* AstepLock2 *)
+          discriminate state.
+        (* AstepUnlock1 *)
+          discriminate state.
+        (* AstepUnlock2 *)
+          discriminate state.
+    (* Aprivate CheckCount, Aprivate (Acc 1) *)
+        destruct H as [ main_lock state ].
+        cases s2_transition.
+        (* AstepN1 *)
+          invert state.
+          invert H.
+          refine (ex_intro _ (S c) (ex_intro _ b (ex_intro _ a (conj _ (conj cnt_b (conj _ _)))))).
+          equality.
+          equality.
+          refine (or_intror (conj (or_intror (or_introl (conj main_lock (conj (eq_refl _) _)))) sum_abc)).
+          exact (ex_intro _ c (eq_refl _)).
+        (* AstepN2 *)
+          invert state.
+          invert H.
+          refine (ex_intro _ c (ex_intro _ b (ex_intro _ (S a) (conj _ (conj cnt_b (conj _ _)))))).
+          equality.
+          rewrite (plus_comm a 1).
+          equality.
+          refine (or_introl (conj (or_intror (or_intror (or_intror (or_intror (or_intror (or_intror
+              (or_intror (conj main_lock (eq_refl _))))))))) _)).
+          simpl in sum_abc.
+          rewrite (plus_n_Sm (c + b) a) in sum_abc.
+          exact sum_abc.
+        (* AstepLock1 *)
+          discriminate state.
+        (* AstepLock2 *)
+          discriminate state.
+        (* AstepUnlock1 *)
+          discriminate state.
+        (* AstepUnlock2 *)
+          discriminate state.
+Qed.
+
 Theorem pdcs2_ok : invariantFor pdcs2_sys pdcs2_correct.
 Proof.
-Admitted.
-
+  refine (invariant_weaken pdcs2_correct pdcs2_ok_complete _).
+  intros s H cnt_eq_0 buf_nil no_lock.
+  destruct H as [a H].
+  destruct H as [b H].
+  destruct H as [c H].
+  destruct H as [cnt_a H].
+  destruct H as [cnt_b H].
+  destruct H as [cnt_c H].
+  cases H.
+  (* We have the equality *)
+    destruct H as [H sum_abc].
+    rewrite cnt_c.
+    rewrite cnt_a in cnt_eq_0.
+    rewrite cnt_eq_0 in sum_abc.
+    rewrite cnt_b in buf_nil.
+    cases b.
+    exact sum_abc.
+    discriminate buf_nil.
+  (* We do not have the equality, but the lock is taken *)
+    destruct H as [H sum_abc].
+    cases H.
+    rewrite (proj1 H) in no_lock.
+    discriminate no_lock.
+    cases H.
+    rewrite (proj1 H) in no_lock.
+    discriminate no_lock.
+    rewrite (proj1 H) in no_lock.
+    discriminate no_lock.
+Qed.
